add:proof of l_jump

theory/JITFlattern.thy
@@ -1,644 +1,9 @@
 theory JITFlattern
 
-imports JITPer_aux x64Semantics JITPer
+imports JITFlattern_aux
 begin
 
-
-type_synonym flat_bpf_prog = "x64_bin \<times> (u64 \<times> nat) list \<times> ((u64\<times>u64) list)"
-
-definition update_l_jump::"(nat \<times> u64 \<times> x64_bin) \<Rightarrow> (u64 \<times> nat) list \<Rightarrow> (u64\<times>u64) list \<Rightarrow> (u64\<times>u64) list" where
-"update_l_jump x l_pc l_jump \<equiv> let l_bin0 = snd(snd x); off = fst(snd x) in
-  if l_bin0!1 = (0x39::u8) then l_jump@ [(of_nat (length l_pc), of_nat (length l_pc) + off)]
-  else l_jump"
-
-fun jitflat_bpf :: "(nat \<times> u64 \<times> x64_bin) list \<Rightarrow> flat_bpf_prog \<Rightarrow> flat_bpf_prog" where
-"jitflat_bpf [] st = st"| 
-"jitflat_bpf ((num,off,l_bin0)#xs) (l_bin,l_pc,l_jump) = (
-  let curr_pc = of_nat (length l_bin) in 
-  let l_jump' = update_l_jump (num,off,l_bin0) l_pc l_jump in
-      jitflat_bpf xs (
-        l_bin@l_bin0,
-        l_pc@[(curr_pc,num)],
-        l_jump')
-)"
-
-lemma jitflat_bpf_induct:
-  "jitflat_bpf (a # l_bin0) (l1, l_pc1, l_jump1) = (l2, l_pc2, l_jump2) \<Longrightarrow> 
-   \<exists> l2' l_pc2' l_jump2'. jitflat_bpf [a] (l1, l_pc1, l_jump1) = (l2', l_pc2', l_jump2') \<and> 
-         jitflat_bpf l_bin0 (l2', l_pc2', l_jump2') = (l2, l_pc2, l_jump2)"
-  by (smt (verit) fst_conv jitflat_bpf.elims list.distinct(1) list.sel(3) nth_Cons_0 snd_conv)
-
-lemma jitflat_bpf_induct2:"jitflat_bpf [a] (l1, l_pc1, l_jump1) = (l2', l_pc2', l_jump2') \<and> 
-         jitflat_bpf l_bin0 (l2', l_pc2', l_jump2') = (l2, l_pc2, l_jump2) \<Longrightarrow> jitflat_bpf (a # l_bin0) (l1, l_pc1, l_jump1) = (l2, l_pc2, l_jump2)"
-  using jitflat_bpf.elims by force
-
-
-lemma jitflat_bpf_induct3:
-  "jitflat_bpf (xs1@xs2) (l1,l_pc1,l_jump1) = (l2, l_pc2, l_jump2) \<Longrightarrow> 
-   \<exists> l2' l_pc2' l_jump2'. jitflat_bpf xs1 (l1,l_pc1,l_jump1) = (l2', l_pc2', l_jump2') \<and> 
-         jitflat_bpf xs2 (l2', l_pc2', l_jump2') = (l2, l_pc2, l_jump2)"
-proof(induct xs1 arbitrary: xs2 l1 l_pc1 l_jump1 l2 l_pc2 l_jump2)
-  case Nil
-  then show ?case by simp
-next
-  case (Cons a xs1)
-  assume a0:"jitflat_bpf ((a#xs1)@xs2) (l1,l_pc1,l_jump1)= (l2, l_pc2, l_jump2)" 
-  have "\<exists> l2' l_pc2' l_jump2'. jitflat_bpf [a] (l1,l_pc1,l_jump1) = (l2', l_pc2', l_jump2')  \<and> jitflat_bpf (xs1@xs2) (l2', l_pc2', l_jump2') = (l2, l_pc2, l_jump2)" 
-    using jitflat_bpf_induct a0 by (metis append_Cons) 
-  then obtain l2' l_pc2' l_jump2' where a1:"jitflat_bpf [a] (l1,l_pc1,l_jump1) = (l2', l_pc2', l_jump2')  \<and> jitflat_bpf (xs1@xs2) (l2', l_pc2', l_jump2') = (l2, l_pc2, l_jump2)" by auto
-  hence "jitflat_bpf (xs1@xs2) (l2', l_pc2', l_jump2') = (l2, l_pc2, l_jump2)" apply rule by simp
-  hence a2:"\<exists> l2'' l_pc2'' l_jump2''. jitflat_bpf xs1 (l2', l_pc2', l_jump2')  = (l2'', l_pc2'', l_jump2'') \<and> 
-         jitflat_bpf xs2 (l2'', l_pc2'', l_jump2'') = (l2, l_pc2, l_jump2) " using Cons by blast
-  then obtain l2'' l_pc2'' l_jump2'' where a3:"jitflat_bpf xs1 (l2', l_pc2', l_jump2')  = (l2'', l_pc2'', l_jump2'') \<and> 
-         jitflat_bpf xs2 (l2'', l_pc2'', l_jump2'') = (l2, l_pc2, l_jump2) " by auto
-  then show ?case using a0 a1 a2 a3 jitflat_bpf_induct2 
-    by (smt (verit) jitflat_bpf.elims jitflat_bpf.simps(1) jitflat_bpf.simps(2) list.sel(3) nth_Cons_0) 
-qed
-
-definition init_second_layer::"x64_bin \<times> (u64 \<times> nat) list \<times> ((u64\<times>u64) list)" where
-"init_second_layer \<equiv> ([],[],[])"
-  
-(*
-lemma list_in_list_prop1:"list_in_list l2 (length l1) (l1@l2@l3) \<Longrightarrow> 
-  list_in_list (l1@l2@l3) (length l1') (l1'@((l1@l2@l3))@l3') \<Longrightarrow>
-  list_in_list l2 (length l1+length l1') (l1'@((l1@l2@l3))@l3')"
-  sorry*)
-
-(*lemma "list_in_list l xpc l_bin \<Longrightarrow> length l = len \<Longrightarrow> l  \<noteq> [] \<Longrightarrow> 
-  idx \<ge>0 \<and> idx < len \<Longrightarrow> l!idx = l_bin!(xpc+idx)"
-  apply(induction l arbitrary:xpc l_bin len idx)
-   apply simp
-  subgoal for a l xpc l_bin len idx 
-    sorry
-  done
-*)
-value "take 0 [1::nat,2]"
-(*value "take 0 ([]::nat)"*)
-value "list_in_list [] 0 [1::nat,2]"
-(*\<forall> idx. idx \<ge>0 \<and> idx < len \<longrightarrow> l!idx = l_bin!(xpc+idx)   l  \<noteq> [] *)
-(*lemma list_in_list_prop4:"list_in_list l 0 l_bin \<Longrightarrow> l_bin \<noteq> [] \<Longrightarrow> take (length l) l_bin = l"
-  sorry*)
- 
-
-lemma list_in_list_prop2:"list_in_list l xpc l_bin \<Longrightarrow> x64_decode x l = x64_decode (xpc+x) l_bin"
-  sorry
-
-
-lemma not_change_prefix_l_bin:
-  "jitflat_bpf l_bin0 (l1,l_pc1,l_jump1) = (l2,l_pc2,l_jump2) \<Longrightarrow> list_in_list l1 0 l2"
-proof(induction l_bin0 arbitrary: l1 l_pc1 l_jump1 l2 l_pc2 l_jump2)
-  case Nil
-  then show ?case using list_in_list_prop
-    by fastforce 
-next
-  case (Cons a l_bin0)
-  have assm1:"jitflat_bpf (a # l_bin0) (l1, l_pc1, l_jump1) = (l2, l_pc2, l_jump2)" using Cons by blast
-  have assm2:"jitflat_bpf l_bin0 (l1, l_pc1, l_jump1) = (l2, l_pc2, l_jump2) \<Longrightarrow> list_in_list l1 (0::nat) l2"
-    using Cons by simp
-
-  have "\<exists> l2' l_pc2' l_jump2'. jitflat_bpf [a] (l1, l_pc1, l_jump1) = (l2', l_pc2', l_jump2')"  by (meson prod_cases3)
-  then obtain l2' l_pc2' l_jump2' where a0:"jitflat_bpf [a] (l1, l_pc1, l_jump1) = (l2', l_pc2', l_jump2')" by auto
-
-  let "?num" = "fst a"
-  let "?off" = "fst (snd a)"
-  let "?l_bin0" = "snd (snd a)"
-  have a3:"jitflat_bpf [(?num,?off,?l_bin0)] (l1, l_pc1, l_jump1) =  (
-    let curr_pc = of_nat (length l1) in 
-    let l_jump' = update_l_jump (?num,?off,?l_bin0) l_pc1 l_jump1 in
-      jitflat_bpf [] (
-        l1@?l_bin0,
-        l_pc1@[(curr_pc,?num)],
-        l_jump'))"  
-    using jitflat_bpf.simps(2) by blast
-  have a4:"l1@?l_bin0 = l2'" using a3
-    by (smt (verit) a0 jitflat_bpf.simps(1) split_pairs) 
-      (*lemma list_in_list_concat: "list_in_list (l1 @ l2) pc l = (list_in_list l1 pc l \<and> list_in_list l2 (pc + length l1) l)"*)
-  have a5:"list_in_list l1 (0::nat) l2'" using a4 list_in_list_concat list_in_list_prop by blast
-  have a6:"jitflat_bpf l_bin0 (l2', l_pc2', l_jump2') = (l2, l_pc2, l_jump2)" using a0 assm1 jitflat_bpf_induct by metis
-
-  have a7:"list_in_list l2' 0 l2" using a6 by (simp add: Cons.IH) 
-  have a6:"list_in_list l1 (0::nat) l2" using a7 a4 list_in_list_concat by blast 
-  then show ?case by simp
-qed
-
-
-lemma not_change_prefix_l_pc:
-  "jitflat_bpf l_bin0 (l1,l_pc1,l_jump1) = (l2,l_pc2,l_jump2) \<Longrightarrow> list_in_list l_pc1 0 l_pc2"
-  proof(induction l_bin0 arbitrary: l1 l_pc1 l_jump1 l2 l_pc2 l_jump2)
-  case Nil
-  then show ?case using list_in_list_prop
-    by fastforce 
-next
-  case (Cons a l_bin0)
-  have assm1:"jitflat_bpf (a # l_bin0) (l1, l_pc1, l_jump1) = (l2, l_pc2, l_jump2)" using Cons by blast
-  have assm2:"jitflat_bpf l_bin0 (l1, l_pc1, l_jump1) = (l2, l_pc2, l_jump2) \<Longrightarrow> list_in_list l_pc1 0 l_pc2"
-    using Cons by simp
-
-  have "\<exists> l2' l_pc2' l_jump2'. jitflat_bpf [a] (l1, l_pc1, l_jump1) = (l2', l_pc2', l_jump2')"  by (meson prod_cases3)
-  then obtain l2' l_pc2' l_jump2' where a0:"jitflat_bpf [a] (l1, l_pc1, l_jump1) = (l2', l_pc2', l_jump2')" by auto
-
-  let "?num" = "fst a"
-  let "?off" = "fst (snd a)"
-  let "?l_bin0" = "snd (snd a)"
-  have a3:"jitflat_bpf [(?num,?off,?l_bin0)] (l1, l_pc1, l_jump1) =  (
-    let curr_pc = of_nat (length l1) in 
-    let l_jump' = update_l_jump (?num,?off,?l_bin0) l_pc1 l_jump1 in
-      jitflat_bpf [] (
-        l1@?l_bin0,
-        l_pc1@[(curr_pc,?num)],
-        l_jump'))"  using jitflat_bpf.simps(2) by blast
-  have a4:"l_pc1@[(of_nat (length l1),?num)] = l_pc2'" using a3
-    by (smt (verit) a0 jitflat_bpf.simps(1) split_pairs) 
-      (*lemma list_in_list_concat: "list_in_list (l1 @ l2) pc l = (list_in_list l1 pc l \<and> list_in_list l2 (pc + length l1) l)"*)
-  have a5:"list_in_list l_pc1 0 l_pc2'" using a4 list_in_list_concat list_in_list_prop by blast
-  have a6:"jitflat_bpf l_bin0 (l2', l_pc2', l_jump2') = (l2, l_pc2, l_jump2)" using a0 assm1 jitflat_bpf_induct by metis
-
-  have a7:"list_in_list l_pc2' 0 l_pc2" using a6 a5 by (simp add: Cons.IH)  
-  have a6:"list_in_list l_pc1 (0::nat) l_pc2" using a7 a4 list_in_list_concat by blast 
-  then show ?case by simp
-qed
-
-lemma l_pc_length_prop:"jitflat_bpf l_bin0 (l1,l_pc1,l_jump1) = (l2,l_pc2,l_jump2) \<Longrightarrow> length l_pc2 = length l_bin0 + length l_pc1"
-proof(induct l_bin0 arbitrary: l1 l_pc1 l_jump1 l2 l_pc2 l_jump2)
-  case Nil
-  then show ?case by simp
-next
-  case (Cons a l_bin0)
-  assume assm0:"jitflat_bpf (a#l_bin0)  (l1,l_pc1,l_jump1) = (l2,l_pc2,l_jump2)"
-  have "\<exists> l2' l_pc2' l_jump2'. jitflat_bpf [a] (l1,l_pc1,l_jump1) = (l2',l_pc2',l_jump2') \<and> jitflat_bpf l_bin0 (l2',l_pc2',l_jump2') = (l2,l_pc2,l_jump2)" using jitflat_bpf_induct assm0 by simp
-  then obtain l2' l_pc2' l_jump2' where a0:"jitflat_bpf [a] (l1,l_pc1,l_jump1) = (l2',l_pc2',l_jump2') \<and> jitflat_bpf l_bin0 (l2',l_pc2',l_jump2') = (l2,l_pc2,l_jump2)" by auto
-  hence a1:"length l_pc2 = length l_bin0 + length l_pc2'" using Cons by blast
-  have a2:"length l_pc2' = 1 + length l_pc1" using a0
-    by (smt (verit) One_nat_def add.commute fst_conv jitflat_bpf.elims length_append list.distinct(1) list.sel(3) list.size(3) list.size(4) plus_1_eq_Suc snd_conv) 
-  hence "length l_pc2 = length(a#l_bin0 )+length l_pc1" using a1 a2 by simp
-  then show ?case by simp
-qed
-
-lemma num_corr:"jitflat_bpf l_bin0 (l1, l_pc1, l_jump1) = (l2,l_pc2,l_jump2) \<Longrightarrow> map snd (drop (length l_pc1) l_pc2) = map fst l_bin0"
-proof(induction l_bin0 arbitrary: l1 l_pc1 l_jump1 l2 l_pc2 l_jump2)
-  case Nil
-  then show ?case by simp
-next
-  case (Cons a l_bin0)
-  have assms1:"jitflat_bpf (a#l_bin0) (l1, l_pc1, l_jump1) = (l2,l_pc2,l_jump2)" using Cons by simp
-
-  have "\<exists> l2' l_pc2' l_jump2'. jitflat_bpf [a] (l1, l_pc1, l_jump1) = (l2', l_pc2', l_jump2') \<and> 
-         jitflat_bpf l_bin0 (l2', l_pc2', l_jump2') = (l2, l_pc2, l_jump2)" 
-    using jitflat_bpf_induct assms1 by (simp add: init_second_layer_def) 
-  then obtain l2' l_pc2' l_jump2' where b4:"jitflat_bpf [a] (l1, l_pc1, l_jump1) = (l2', l_pc2', l_jump2') \<and> 
-         jitflat_bpf l_bin0 (l2', l_pc2', l_jump2') = (l2, l_pc2, l_jump2)" by auto
- 
-  have b5:"list_in_list l_pc1 0 l_pc2" using not_change_prefix_l_pc assms1 by blast
-  have b5_1:"list_in_list l_pc2' 0 l_pc2" using not_change_prefix_l_pc b4 by blast
-
-  have b6:"(list_in_list (drop (length l_pc1) l_pc2) (length l_pc1) l_pc2)"
-    using b5 list_in_list_concat list_in_list_prop
-    using list_in_list.simps(1)
-    by (metis (no_types, lifting) append.right_neutral append_take_drop_id drop_eq_Nil2 gen_length_def gen_length_def length_code length_code length_take min.commute nat_le_linear) 
-
-  have b7:"map snd (drop (length l_pc2') l_pc2) = map fst l_bin0" using b4 Cons by blast
-
-  have "jitflat_bpf [a] (l1, l_pc1, l_jump1) = (
-      jitflat_bpf [] (
-        l1@(snd(snd a)),
-        l_pc1@[(of_nat(length l1), fst a)],
-        update_l_jump a l_pc1 l_jump1))" using b4
-    by (metis jitflat_bpf.simps(2) prod.collapse) 
-
-  hence b8:"l_pc2' = l_pc1@[(of_nat(length l1), fst a)]" using b4 by force
-  hence "drop (length l_pc1) l_pc2' = [(of_nat(length l1), fst a)]" by auto
-
-  have "length l_pc1 + 1 = length l_pc2'" using b8 by simp
-  hence b10:"(drop (length l_pc1) l_pc2) = (of_nat(length l1), fst a) # (drop (length l_pc2') l_pc2) "
-    using b8 b5_1 l_pc_length_prop
-    by (metis (no_types, lifting) Cons_nth_drop_Suc ab_semigroup_add_class.add_ac(1) add.right_neutral 
-        add_Suc_right assms1 gen_length_def length_Cons length_code less_add_Suc2 list_in_list.simps(2) list_in_list_concat plus_1_eq_Suc) 
-    
-  hence"map snd (drop (length l_pc1) l_pc2) = fst a # map fst l_bin0" using b7 b8 by force 
-  hence " map snd (drop (length l_pc1) l_pc2) = map fst (a # l_bin0)" by simp
-
-  then show ?case by simp
-qed
-
-lemma flattern_lbin:
-  assumes a0:"l_bin0!0=(num,off,l)" and
-   a1:"unat pc < length l_bin0 \<and> unat pc \<ge> 0" and
-   a2:"jitflat_bpf l_bin0 (l1,l_pc1,l_jump1) = (l2,l_pc2,l_jump2)" and
-   a3:"fst (l_pc2 ! (length l_pc1) ) = xpc"
- shows "list_in_list l (unat xpc) l2"
-proof-
-  let "?xs" = "tl l_bin0"
-  have b0:"jitflat_bpf ((num,off,l)#?xs) (l1,l_pc1,l_jump1) = (
-  let curr_pc = of_nat (length l1) in 
-  let l_jump' = update_l_jump (num,off,l) l_pc1 l_jump1 in  
-      jitflat_bpf ?xs (l1@l, l_pc1@[(curr_pc,num)], l_jump'))" using a1 by auto
-
-  have b1:"(num,off,l)#?xs = l_bin0" using a0 a1
-    by (metis Nitpick.size_list_simp(2) hd_conv_nth list.collapse not_less0) 
-  have c0:"jitflat_bpf ((num,off,l)#?xs) (l1,l_pc1,l_jump1) =  (jitflat_bpf ?xs (l1@l, l_pc1@[(of_nat (length l1),num)], update_l_jump (num,off,l) l_pc1 l_jump1))"
-      using b0 by auto
-  have c1_0:"jitflat_bpf ?xs (l1@l, l_pc1@[((of_nat (length l1)),num)],update_l_jump (num,off,l) l_pc1 l_jump1) = (l2,l_pc2,l_jump2)" using c0 a2 b1 by simp 
-  have c1_1:"list_in_list (l_pc1@[((of_nat (length l1)),num)]) 0 l_pc2" using c1_0 not_change_prefix_l_pc by simp
-  have c1_2:"list_in_list [((of_nat (length l1)),num)] (length l_pc1) l_pc2" using c1_1 list_in_list_concat by force
-  have c1:"l_pc2! (length(l_pc1)) = ((of_nat (length l1)),num)" using not_change_prefix_l_pc c1_2 by simp
-
-  have c2:"xpc = of_nat (length l1)" using c1 a3 by simp
-
-  have c3_1:"list_in_list (l1@l) 0 l2" using c1_0 not_change_prefix_l_bin by blast
-  have c3_2:"list_in_list l (length l1) l2" using c3_1 list_in_list_concat by (metis plus_nat.add_0) 
-  have c3_3:"unat (of_nat (length l1)) = (length l1)" sorry
-  have c3:"list_in_list l (unat xpc) l2" using c2 c3_2 c3_3 by metis
-    then show ?thesis by simp    
-  qed
-
-
-(*lemma flattern_l_bin0:
-  assumes a0:"l_bin0!(unat pc)=(num,off,l)" and
-   a1:"l_bin0 \<noteq> []" and
-   a2:"jitflat_bpf l_bin0 (l1,l_pc1,l_jump1) = (l2,l_pc2,l_jump2)" and
-   a3:"fst (l_pc2 ! (length l_pc1 + (unat pc))) = xpc"
- shows "list_in_list l (unat xpc) l2"
-  sorry*)
-
-(*lemma flattern_l_bin0:
-  "l_bin0!(unat pc)=(num,off,l) \<Longrightarrow>
-   unat pc < length l_bin0 \<and> unat pc \<ge> 0 \<Longrightarrow>
-   jitflat_bpf l_bin0 (l1,l_pc1,l_jump1) = (l2,l_pc2,l_jump2) \<Longrightarrow>
-   fst (l_pc2 ! (length l_pc1 + (unat pc))) = xpc \<Longrightarrow>
-   list_in_list l (unat xpc) l2"
-proof(induct l_bin0 arbitrary: pc num off l l1 l_pc1 l_jump1 l2 l_pc2 l_jump2 xpc)
-  case Nil
-  then show ?case by simp
-next
-  case (Cons a l_bin0)
-  assume assm0:"l_bin0!(unat pc)=(num,off,l)" and
-   assm1:"unat pc < length l_bin0 \<and> unat pc \<ge> 0" and
-   assm2:"jitflat_bpf l_bin0 (l1,l_pc1,l_jump1) = (l2,l_pc2,l_jump2)" and
-   assm3:"fst (l_pc2 ! (length l_pc1 + (unat pc))) = xpc"
-  then show ?case sorry
-qed*)
-
-
-lemma flattern_l_bin0:
-  "l_bin0!(unat pc)=(num,off,l) \<Longrightarrow>
-   unat pc < length l_bin0 \<and> unat pc \<ge> 0 \<Longrightarrow>
-   jitflat_bpf l_bin0 init_second_layer = (l2,l_pc2,l_jump2) \<Longrightarrow>
-   fst (l_pc2 ! (unat pc)) = xpc \<Longrightarrow>
-   list_in_list l (unat xpc) l2"
-proof-
-  assume assm0:"l_bin0!(unat pc)=(num,off,l)" and
-   assm1:"unat pc < length l_bin0 \<and> unat pc \<ge> 0" and
-   assm2:"jitflat_bpf l_bin0 init_second_layer = (l2,l_pc2,l_jump2)" and
-   assm3:"fst (l_pc2 ! (unat pc)) = xpc"
-
-  let "?prefix" = "take (unat pc) l_bin0"
-  let "?suffix" = "drop (unat pc+1) l_bin0"
-  have "?prefix@[(num,off,l)]@?suffix= l_bin0" using append_take_drop_id assm0
-    by (metis (no_types, opaque_lifting) Cons_nth_drop_Suc append_eq_Cons_conv assm1 drop_0 drop_Suc_Cons drop_drop plus_1_eq_Suc self_append_conv2)  
-  hence "?prefix@((num,off,l)#?suffix)= l_bin0" by simp
-
-  hence "\<exists> l2' l_pc2' l_jump2'. jitflat_bpf ?prefix init_second_layer = (l2', l_pc2', l_jump2') \<and> 
-         jitflat_bpf ((num,off,l)#?suffix) (l2', l_pc2', l_jump2') = (l2, l_pc2, l_jump2)" 
-    using init_second_layer_def jitflat_bpf_induct3 by (metis assm2) 
-
-  then obtain l2' l_pc2' l_jump2' where c0:"jitflat_bpf ?prefix init_second_layer = (l2', l_pc2', l_jump2') \<and> 
-         jitflat_bpf ((num,off,l)#?suffix) (l2', l_pc2', l_jump2') = (l2, l_pc2, l_jump2)" by auto
-
-  have c1:"jitflat_bpf ((num,off,l)#?suffix) (l2', l_pc2', l_jump2') = (
-    let l_jump' = update_l_jump (num,off,l) l_pc2' l_jump2' in
-        jitflat_bpf ?suffix (
-          l2'@l,
-          l_pc2'@[(of_nat(length l2'),num)],
-          l_jump')
-  )" using assm2 init_second_layer_def of_nat_def c0 using jitflat_bpf.simps(2) by presburger   
-
-  have c2:"list_in_list l_pc2' 0 l_pc2" using not_change_prefix_l_pc c0 c1 by blast
-
-  have c3:"(l_pc2 ! (unat pc)) = (of_nat(length l2'),num)" using c2 l_pc_length_prop
-    by (smt (z3) Cons_nth_drop_Suc Suc_eq_plus1 ab_semigroup_add_class.add_ac(1) add.commute assm1 assm2 c0 c1 diff_add_inverse diff_diff_cancel init_second_layer_def length_drop less_or_eq_imp_le list.size(3) list.size(4) list_in_list.simps(2) list_in_list_concat not_change_prefix_l_pc) 
-    
-  have c4:"fst (l_pc2 ! (unat pc)) = (of_nat(length l2'))" using c3 by auto
-  
-  have c6:"list_in_list l (length l2') l2" using c0 c1 not_change_prefix_l_bin
-    by (metis (mono_tags, lifting) list_in_list_concat plus_nat.add_0) 
-  hence c7:"list_in_list l (unat(of_nat(length l2'))) l2" sorry
-  
-  have "list_in_list l (unat(fst (l_pc2 ! (unat pc)))) l2" using c7 c4 by metis 
-     then show ?thesis using assm3 by force 
-   qed
-
-
-lemma flattern_num:
-  "l_bin0!(unat pc)=(num,off,l) \<Longrightarrow>
-   unat pc < length l_bin0 \<and> unat pc \<ge> 0 \<Longrightarrow>
-   jitflat_bpf l_bin0 init_second_layer = (l2,l_pc2,l_jump2) \<Longrightarrow>
-   snd (l_pc2!(unat pc)) = num"
-proof(induct l_bin0 arbitrary: pc num off l l2 l_pc2 l_jump2)
-  case Nil 
-  have "length l_bin0 = 0" using Nil by simp
-  then show ?case using Nil.prems(2) by auto  
-    
-next
-  case (Cons a l_bin0)
-  then show ?case
-  proof-
-  have assm1:"(a # l_bin0) ! unat pc = (num, off, l)" using Cons by simp
-  have assm2:"unat pc < length (a # l_bin0) \<and> (0::nat) \<le> unat pc" using Cons by simp
-  have assm3:"jitflat_bpf (a # l_bin0) init_second_layer = (l2, l_pc2, l_jump2)" using Cons by simp
-  
-  have "l_bin0 ! unat pc = (num, off, l) \<Longrightarrow> unat pc < length l_bin0 \<and> (0::nat) \<le> unat pc \<Longrightarrow>
-    jitflat_bpf l_bin0 init_second_layer = (l2, l_pc2, l_jump2) \<Longrightarrow> snd (l_pc2 ! unat pc) = num"
-    using Cons by simp
-
-  have a0:"unat pc = 0 \<or> unat pc \<ge> 1" by auto
-  show ?thesis
-  proof(cases "unat pc = 0")
-    case True
-      have "snd (l_pc2!(unat pc)) = num" using not_change_prefix_l_pc True
-        by (smt (verit, ccfv_threshold) append_Nil assm1 assm3 init_second_layer_def jitflat_bpf.simps(2) list_in_list.simps(2) nth_Cons_0 prod.collapse prod.inject)
-      then show ?thesis by simp
-  next
-    case False
-      have b0:"unat pc \<ge>1" using False a0 by simp
-      let "?pc" = "unat pc -1"
-      have b1:"?pc < length l_bin0 \<and> (0::nat) \<le> ?pc" using assm2 b0 using diff_le_self order_le_less_trans by simp
-      let "?x" = "tl l_bin0"
-      have b2:"l_bin0 ! ?pc = (num, off, l)" using assm1
-        by (simp add: False order_neq_le_trans) 
-      
-      have b2_1:"jitflat_bpf (a#l_bin0) init_second_layer = (
-        jitflat_bpf l_bin0 (
-          []@(snd(snd a)),
-          []@[(0, fst a)],
-          update_l_jump a [] []))" using init_second_layer_def 
-        by (metis jitflat_bpf.simps(2) list.size(3) prod.exhaust_sel semiring_1_class.of_nat_0) 
-  
-      hence b2_2:"jitflat_bpf (a#l_bin0) init_second_layer = jitflat_bpf l_bin0 ((snd(snd a)),[(0, fst a)],update_l_jump a [] [])" by auto
-      
-      have "\<exists> l2' l_pc2' l_jump2'. jitflat_bpf l_bin0 init_second_layer = (l2',l_pc2',l_jump2') " by (metis surj_pair)
-      then obtain l2' l_pc2' l_jump2' where b3_1:"jitflat_bpf l_bin0 init_second_layer = (l2',l_pc2',l_jump2')" by auto
-      (*have b4:"l_bin0 \<noteq> []" sorry*)
-  
-        have b3:"snd (l_pc2'! ?pc) = num" using Cons False using b0 b1 b2 b3_1 
-        by (metis (mono_tags, lifting) order_neq_le_trans unat_gt_0 unat_minus_one) 
-  
-      have c0:"map snd l_pc2' = map fst l_bin0" using num_corr b3_1 init_second_layer_def
-        by (metis append_Nil append_eq_conv_conj) 
-      have c1:"map snd l_pc2 = map fst (a#l_bin0)" using num_corr assm3 init_second_layer_def
-        by (metis drop0 list.size(3)) 
-      (*have c2:"l_pc2 \<noteq> []" using c1 by auto
-      have c3:"l_pc2' \<noteq> []" sorry*)
-      (*have c2:"map fst (a#l_bin0) = fst a # map fst l_bin0" by auto*)
-  
-      (*have "\<exists> l2'' l_pc2'' l_jump2''. jitflat_bpf [a] init_second_layer = l2'' l_pc2'' l_jump2''" by blast
-      then obtain l2'' l_pc2'' l_jump2'' where "jitflat_bpf [a] init_second_layer = l2'' l_pc2'' l_jump2''" by auto
-      have b2_3:"list_in_list [(0, fst a)] 0 l_pc2" using not_change_prefix_l_pc b2_2 assm3 by metis
-      have b2_4:"l_pc2!0 = (0, fst a)" using b2_3 by auto*)
-      have "map snd l_pc2 = (fst a)#(map snd l_pc2')" using c0 c1 b2_2 by auto
-        (*using assm3 b3 init_second_layer_def not_change_prefix_l_pc b2_2 b2_3 b2_4 num_corr *)
-      hence "(map snd l_pc2)!(unat pc) = (map snd l_pc2')!?pc" using b3 False by auto
-      hence "snd (l_pc2! unat pc) = num" 
-        using b3 False by (metis assm2 b1 c0 c1 map_equality_iff nth_map)
-      then show ?thesis by auto  
-    qed
-  qed
-qed
-
-(*
-lemma flattern_num:
-  assumes a0:"l_bin0!(unat pc)=(num,off,l)" and
-   a1:"l_pc2 \<noteq> []" and
-   a2:"jitflat_bpf l_bin0 (l1,l_pc1,l_jump1) = (l2,l_pc2,l_jump2)" and
-   a3:"unat pc < length l_bin0 \<and> unat pc \<ge> 0"
- shows "snd (l_pc2!(length l_pc1 + unat pc)) = num"
-  sorry*)
-
-fun find_target_pc_in_l_pc :: "((u64\<times>u64) list) \<Rightarrow> u64 \<Rightarrow> u64 option" where
-"find_target_pc_in_l_pc [] _ = None" |
-"find_target_pc_in_l_pc ((x, y)#xs) pc = (
-  if x = pc then Some y
-  else find_target_pc_in_l_pc xs pc
-)"
-
-
-definition flat_bpf_one_step :: "flat_bpf_prog \<Rightarrow> hybrid_state \<Rightarrow> hybrid_state" where
-"flat_bpf_one_step lp st = (
-  let (l_bin,l_pc,l_jump) = lp in
-  let (pc, xst) = st in
-  let num = snd (l_pc!(unat pc)) in 
-    (case xst of
-    Stuck \<Rightarrow> (pc, Stuck) |
-    Next xpc rs m ss \<Rightarrow> (
-        if l_bin!(xpc+1) = (0x39::u8) then \<comment>\<open> TODO: if the first byte is the opcode of cmp? \<close>
-          \<comment>\<open> case: BPF JMP \<close>
-          (case x64_sem 1 l_bin (Next xpc rs m ss) of
-          Stuck \<Rightarrow> (pc, Stuck) | \<comment>\<open> if one step error, stop, it should be impossible \<close>
-          Next xpc1 rs1 m1 ss1 \<Rightarrow> (
-            if rs1 (CR ZF) = 1 then \<comment>\<open> must JUMP \<close>
-              (case find_target_pc_in_l_pc l_jump pc of
-              None \<Rightarrow> (pc, Stuck) |
-              Some npc \<Rightarrow>
-                (npc, (Next (unat (fst (l_pc!(unat npc)))) rs1 m1 ss1))) \<comment>\<open> go to the target address in the jited x64 binary \<close>
-            else \<comment>\<open> donot JUMP \<close>
-              (pc+1, xst)
-          ))
-         else
-          \<comment>\<open> case: NOT BPF JMP \<close>
-          (pc+1, x64_sem num l_bin (Next xpc rs m ss))
-)))"
-
-fun flat_bpf_sem :: "nat \<Rightarrow> flat_bpf_prog \<Rightarrow> hybrid_state \<Rightarrow> hybrid_state" where
-"flat_bpf_sem 0 _ (pc,st) = (pc,st)" |
-"flat_bpf_sem (Suc n) lt (pc, xst) = (
-   let pair = flat_bpf_one_step lt (pc, xst) in
-    flat_bpf_sem n lt pair
-)"
-
-
-definition match_state1::"outcome \<Rightarrow> outcome \<Rightarrow> bool" where
-  "match_state1 fxst xxst \<equiv> 
-  (case fxst of (Next xst xrs xm xss) \<Rightarrow>
-    (case xxst of (Next xst1 xrs1 xm1 xss1) \<Rightarrow> 
-     xrs = xrs1 \<and> xm = xm1 \<and> xss = xss1 |
-                   _ \<Rightarrow> False)|
-                 _ \<Rightarrow> False)"
-
-definition match_state::"hybrid_state \<Rightarrow> hybrid_state \<Rightarrow> bool" where
-  "match_state fxst xxst \<equiv> 
-  (case fxst of (pc,Next xst xrs xm xss) \<Rightarrow>
-    (case xxst of (pc1,Next xst1 xrs1 xm1 xss1) \<Rightarrow> 
-      pc = pc1 \<and> match_state1 (Next xst1 xrs1 xm1 xss1) (Next xst xrs xm xss)  |
-                   _ \<Rightarrow> False)|
-                 _ \<Rightarrow> False)"
-(*x64_decode 0 l = x64_decode xpc l
-xxst = Next xpc1 xrs1 xm1 xss1 \<Longrightarrow>
-   fxst = Next xpc2 xrs2 xm2 xss2 \<Longrightarrow>
-xrs1 = xrs2 \<and> xm1 = xm2 \<and> xss1 = xss2*)
-
-lemma err_is_still_err2:"x64_sem n l Stuck = xst' \<Longrightarrow> xst' = Stuck "
-  apply(induct n, simp)
-  using perir_step_def
-  by auto
-
-lemma intermediate_step_is_ok2:
-  "x64_sem n l xst = xst' \<Longrightarrow> n \<ge> 0 \<Longrightarrow> xst' \<noteq> Stuck \<Longrightarrow> \<exists> xpc xrs xm xss. xst = (Next xpc xrs xm xss)"
-  apply(induct n arbitrary: l xst xst')
-   apply simp apply (meson outcome.exhaust) 
-  using err_is_still_err2 by (metis outcome.exhaust)
-
-lemma list_in_list_prop3:"x64_sem num l_bin (Next (xpc+x) xrs xm xss) = fxst \<Longrightarrow>
-   x64_sem num l (Next x xrs xm xss) = xxst \<Longrightarrow>
-   list_in_list l xpc l_bin \<Longrightarrow>
-   xxst \<noteq> Stuck \<Longrightarrow>
-   match_state1 xxst fxst"
-proof(induction num arbitrary:l_bin xpc x xrs xm xss fxst l xrs xm xss xxst)
-  case 0
-  then show ?case using match_state1_def by auto
-next
-  case (Suc num)
-  assume assm0:"x64_sem (Suc num) l_bin (Next (xpc+x) xrs xm xss) = fxst" and
-      assm1:"x64_sem (Suc num) l (Next x xrs xm xss) = xxst" and
-      assm2:"list_in_list l xpc l_bin" and
-      assm3:"xxst \<noteq> Stuck"
-
-  have "x64_sem 1 l_bin (Next (xpc+x) xrs xm xss) = 
-              (case x64_decode (xpc+x) l_bin of
-                None \<Rightarrow> Stuck |
-                Some (sz, ins) \<Rightarrow>
-             x64_sem 0 l_bin (exec_instr ins sz (xpc+x) xrs xm xss))" by simp
-  hence b0:"x64_sem 1 l_bin (Next (xpc+x) xrs xm xss) = 
-              (case x64_decode (xpc+x) l_bin of
-                None \<Rightarrow> Stuck |
-                Some (sz, ins) \<Rightarrow>
-             (exec_instr ins sz (xpc+x) xrs xm xss))"
-    using x64_sem.simps(1) by presburger 
-
-  have "x64_sem 1 l (Next x xrs xm xss) = 
-              (case x64_decode x l of
-                None \<Rightarrow> Stuck |
-                Some (sz, ins) \<Rightarrow>
-             x64_sem 0 l (exec_instr ins sz x xrs xm xss))" by simp
-  hence d0:"x64_sem 1 l (Next x xrs xm xss) = 
-              (case x64_decode x l of
-                None \<Rightarrow> Stuck |
-                Some (sz, ins) \<Rightarrow>
-             (exec_instr ins sz x xrs xm xss))"
-    using x64_sem.simps(1) by presburger  
-  have a0:"x64_decode x l = x64_decode (xpc+x) l_bin" using assm2 list_in_list_prop2
-    by (metis add_0 list_in_list.simps(1))
-
-
-  have d1_0:"x64_sem 1 l (Next x xrs xm xss) \<noteq> Stuck" 
-    using assm3 assm1 by (metis err_is_still_err2 plus_1_eq_Suc x64_sem_add) 
-  hence d1_1:"x64_decode x l \<noteq> None" using d0 by(cases "x64_decode x l",simp_all)
-  hence "\<exists> sz ins. x64_decode x l = Some (sz,ins)" by simp
-  then obtain sz ins where d1_2:"x64_decode x l = Some (sz,ins)" by auto
-  hence d1:"x64_sem 1 l (Next x xrs xm xss) = (exec_instr ins sz x xrs xm xss)" 
-    using d0 by fastforce 
-
-  hence "\<exists> xpc'' xrs'' xm'' xss''. exec_instr ins sz x xrs xm xss = Next xpc'' xrs'' xm'' xss''" 
-    using d1 outcome.exhaust d1_0 by metis
-  then obtain xpc'' xrs'' xm'' xss'' where d2:"exec_instr ins sz x xrs xm xss = Next xpc'' xrs'' xm'' xss''" by auto
-
-  have b1:"x64_sem 1 l_bin (Next (xpc+x) xrs xm xss) = (exec_instr ins sz (xpc+x) xrs xm xss)"
-    using d1_1 d1_2 b0 a0 by simp
-  (* have "x64_sem 1 l_bin (Next (xpc+x) xrs xm xss) \<noteq> Stuck" using intermediate_step_is_ok2 sorry*)
-  thus ?case
-  proof(cases "x64_sem 1 l_bin (Next (xpc+x) xrs xm xss) \<noteq> Stuck")
-    case True
-    hence "\<exists> xpc' xrs' xm' xss'. exec_instr ins sz (xpc+x) xrs xm xss = Next xpc' xrs' xm' xss'"
-       using b1 outcome.exhaust by metis
-    then obtain xpc' xrs' xm' xss' where b2:"exec_instr ins sz (xpc+x) xrs xm xss = Next xpc' xrs' xm' xss'" by auto
-            (*xpc' = xpc1 + sz \<and> xpc'' = 0 + sz \<and> *)
-    have a1:"xrs'' = xrs' \<and> xm'' = xm' \<and> xss'' = xss'"
-              using b2 d2 apply(unfold exec_instr_def)
-              apply(cases ins,simp_all)
-              subgoal for x7 apply(unfold exec_push_def Let_def)
-                apply(cases "storev M64 xm (Vptr sp_block (xrs (IR SP) - u64_of_memory_chunk M64)) (Vlong (xrs (IR x7)))",simp_all)
-                done
-              subgoal for x8 apply(unfold exec_pop_def Let_def)
-                apply(cases "loadv M64 xm (Vptr sp_block (xrs (IR SP)))",simp_all)
-                subgoal for a apply(cases a,simp_all)
-                  done
-                done
-              subgoal for x131 x132 apply(cases "eval_testcond x131 xrs",simp_all)
-                subgoal for a 
-                  by (metis outcome.inject) 
-                done
-              subgoal for x151 x152 x153
-                apply(unfold exec_store_def,simp_all)
-                apply(cases "storev x153 xm (Vlong (eval_addrmode64 x151 xrs)) (Vlong (xrs (IR x152)))",simp_all)
-                done
-              subgoal for x201 x202 x203 
-                apply(unfold exec_load_def,simp_all)
-                apply(cases "loadv x203 xm (Vlong (eval_addrmode64 x202 xrs))",simp_all)
-                subgoal for a apply(cases a,simp_all)
-                  done
-                done
-              subgoal for x21a 
-                apply(unfold exec_call_def,simp_all)
-                done
-              done
-    have a2:"xpc'' = x + sz \<and> xpc'= xpc + x + sz" sorry
-  
-    let "?x" = "sz+x"
-  
-    have a3:"match_state1 (Next ?x xrs' xm' xss') (Next (?x + xpc) xrs' xm' xss')"
-      using a1 apply(unfold match_state1_def)
-      apply(cases "Next ?x xrs' xm' xss'",simp_all)
-      done
-  
-    (*hence a4:"match_state1 (x64_sem 1 l (Next x xrs xm xss)) (x64_sem 1 l_bin (Next (xpc+x) xrs xm xss))" sorry*)
-  
-    have "x64_sem num l_bin (Next (xpc+x) xrs xm xss) = fxst \<Longrightarrow> 
-    x64_sem num l (Next x xrs xm xss) = xxst \<Longrightarrow> 
-    list_in_list l xpc l_bin \<Longrightarrow> 
-    match_state1 xxst fxst" using Suc by simp
-  
-    have a5:"x64_sem num l_bin (Next (xpc+?x) xrs' xm' xss') = fxst" 
-      using a2 a1
-      by (metis Suc.prems(1) ab_semigroup_add_class.add_ac(1) add.commute b1 b2 plus_1_eq_Suc x64_sem_add) 
-    have a6:"x64_sem num l (Next ?x xrs' xm' xss') = xxst" using a1 a2
-      by (metis Suc.prems(2) add.commute d1 d2 plus_1_eq_Suc x64_sem_add) 
-    have "match_state1 xxst fxst" using a6 a5 assm2 Suc by blast
-    then show ?thesis by simp
-  next
-    case False
-    have "exec_instr ins sz (xpc+x) xrs xm xss = Stuck" using b1 False by simp
-    hence "exec_instr ins sz x xrs xm xss = Stuck" 
-      apply(unfold exec_instr_def)
-      apply(cases ins,simp_all)
-              subgoal for x7 apply(unfold exec_push_def Let_def)
-                apply(cases "storev M64 xm (Vptr sp_block (xrs (IR SP) - u64_of_memory_chunk M64)) (Vlong (xrs (IR x7)))",simp_all)
-                done
-              subgoal for x8 apply(unfold exec_pop_def Let_def)
-                apply(cases "loadv M64 xm (Vptr sp_block (xrs (IR SP)))",simp_all)
-                subgoal for a apply(cases a,simp_all)
-                  done
-                done
-              subgoal for x131 x132 apply(cases "eval_testcond x131 xrs",simp_all)
-                subgoal for a
-                  by (metis outcome.distinct(1))          
-                done
-              subgoal for x151 x152 x153
-                apply(unfold exec_store_def,simp_all)
-                apply(cases "storev x153 xm (Vlong (eval_addrmode64 x151 xrs)) (Vlong (xrs (IR x152)))",simp_all)
-                done
-              subgoal for x201 x202 x203 
-                apply(unfold exec_load_def,simp_all)
-                apply(cases "loadv x203 xm (Vlong (eval_addrmode64 x202 xrs))",simp_all)
-                subgoal for a apply(cases a,simp_all)
-                  done
-                done
-              subgoal for x21a 
-                apply(unfold exec_call_def,simp_all)
-                done
-              done
-    then show ?thesis using d2 by simp 
-  qed
-qed
- 
-lemma one_step_equiv:
+lemma one_step_equiv_layer1:
   assumes a0:"flat_bpf_sem 1 (l_bin,l_pc,l_jump) (pc, fxst) = fxst'" and
    a1:"jitflat_bpf lt init_second_layer = (l_bin,l_pc,l_jump)" and
    a2:"perir_sem 1 lt (pc,xxst) = xxst'" and
@@ -646,33 +11,45 @@ lemma one_step_equiv:
    a4:"lt \<noteq> []" and
    a5:"match_state (pc, xxst) (pc, fxst)" and
    a6:"snd xxst' \<noteq> Stuck" and
-   a7:"unat pc < length lt \<and> unat pc \<ge> 0"
+   a7:"unat pc < length lt \<and> unat pc \<ge> 0" and 
+   a8:"well_formed_prog lt" and
+   a9:"snd fxst' \<noteq> Stuck"
   shows"match_state xxst' fxst'"
 proof-
   have "\<exists> xpc1. fxst = Next xpc1 xrs xm xss" using a3 a5 
     apply(unfold match_state_def match_state1_def) 
     apply(cases fxst,simp_all)
     done
-  then obtain xpc1 where a6:"fxst = Next xpc1 xrs xm xss" by auto
+  then obtain xpc1 where a10:"fxst = Next xpc1 xrs xm xss" by auto
 
   let "?curr_ins" = "lt!(unat pc)"
   let "?num" = "fst (lt!(unat pc))"
   let "?off" = "fst (snd (lt!(unat pc)))"
   let "?l" = "snd (snd (lt!(unat pc)))"
+  (*have "\<exists> num off l. (num, off, l) = lt!(unat pc)" using a4 a7 by (metis prod.exhaust_sel) 
+  then obtain num off l where b0_0:"(num, off, l) = lt!(unat pc)" by auto*)
   have b0:"(?num, ?off, ?l) = lt!(unat pc)" by simp
  
   let "?xpc" = "fst (l_pc ! (unat pc))"
   have c0:"list_in_list ?l (unat ?xpc) l_bin" 
-    using flattern_l_bin0 init_second_layer_def a1 b0 a4 a7 by metis
-  have c1:"unat ?xpc= xpc1" sorry
+    using flattern_l_bin0 init_second_layer_def a1 b0 a4 a7 a8 by metis
+  let "?prefix" = "take (unat pc) lt"
+  let "?suffix" = "drop (unat pc+1) lt"
+  have "?prefix@[(?num,?off,?l)]@?suffix= lt" using append_take_drop_id init_second_layer_def
+    by (simp add: Cons_nth_drop_Suc a7) 
+  hence "?prefix@((?num,?off,?l)#?suffix)= lt" by simp
 
-  have "fxst' = flat_bpf_one_step (l_bin,l_pc,l_jump) (pc, Next xpc1 xrs xm xss)" using a0 a6
+
+  have "fxst' = flat_bpf_one_step (l_bin,l_pc,l_jump) (pc, Next xpc1 xrs xm xss)" using a0 a10
     by (metis One_nat_def flat_bpf_sem.simps(1) flat_bpf_sem.simps(2) old.prod.exhaust) 
   hence c2:"fxst' = (
+  if unat pc \<ge> length l_pc \<or> unat pc < 0 then (pc,Stuck) else 
   let num = snd (l_pc!(unat pc)) in 
+  let old_xpc = unat (fst (l_pc!(unat pc))) in 
+        if xpc1 \<noteq> old_xpc then (pc, Stuck) else 
         if l_bin!(xpc1+1) = (0x39::u8) then \<comment>\<open> TODO: if the first byte is the opcode of cmp? \<close>
           \<comment>\<open> case: BPF JMP \<close>
-          (case x64_sem 1 l_bin (Next xpc1 xrs xm xss) of
+          (case x64_sem num l_bin (Next xpc1 xrs xm xss) of
           Stuck \<Rightarrow> (pc, Stuck) | \<comment>\<open> if one step error, stop, it should be impossible \<close>
           Next xpc1 rs1 m1 ss1 \<Rightarrow> (
             if rs1 (CR ZF) = 1 then \<comment>\<open> must JUMP \<close>
@@ -681,15 +58,36 @@ proof-
               Some npc \<Rightarrow>
                 (npc, (Next (unat (fst (l_pc!(unat npc)))) rs1 m1 ss1))) \<comment>\<open> go to the target address in the jited x64 binary \<close>
             else \<comment>\<open> donot JUMP \<close>
-              (pc+1, fxst)
+              (pc+1, Next xpc1 rs1 m1 ss1)
           ))
          else
           \<comment>\<open> case: NOT BPF JMP \<close>
           (pc+1, x64_sem num l_bin (Next xpc1 xrs xm xss)))" 
     apply(unfold flat_bpf_one_step_def Let_def) 
-    using a3 a6 apply(cases "Next xpc1 xrs xm xss",simp_all)
-    subgoal for x11 by meson  
+    using a3 a10 apply(cases "Next xpc1 xrs xm xss",simp_all)
+    (*subgoal for x11 by meson *)
     done
+
+ (* hence "\<exists> l2' l_pc2' l_jump2'. jitflat_bpf ?prefix init_second_layer = (l2', l_pc2', l_jump2') \<and> 
+         jitflat_bpf ((?num,?off,?l)#?suffix) (l2', l_pc2', l_jump2') = (l_bin,l_pc,l_jump)" 
+    using init_second_layer_def jitflat_bpf_induct3 by (metis a1) 
+
+  then obtain l2' l_pc2' l_jump2' where e0:"jitflat_bpf ?prefix init_second_layer = (l2', l_pc2', l_jump2') \<and> 
+         jitflat_bpf ((?num,?off,?l)#?suffix) (l2', l_pc2', l_jump2') = (l_bin,l_pc,l_jump)" by auto
+
+  have e1:"jitflat_bpf ((?num,?off,?l)#?suffix) (l2', l_pc2', l_jump2') = (
+    let l_jump' = update_l_jump (?num,?off,?l) l_pc2' l_jump2' in
+        jitflat_bpf ?suffix (
+          l2'@?l,
+          l_pc2'@[(of_nat(length l2'),?num)],
+          l_jump')
+  )" using a1 init_second_layer_def of_nat_def using jitflat_bpf.simps(2) by presburger   
+
+  have e2:"list_in_list l_pc2' 0 l_pc" using not_change_prefix_l_pc e0 e1 by blast
+
+  have e3:"fst (l_pc ! (unat pc)) = of_nat(length l2')" using e2 l_pc_length_prop a1 a7 b0 e0 e1 a4 init_second_layer_def not_change_prefix_l_pc sorry*)
+
+  have c1:"unat ?xpc= xpc1" using a8 c2 a9 by (smt (verit, ccfv_SIG) snd_conv) 
 
   have "xxst' = perir_step lt (pc,xxst)" using a2 by (metis One_nat_def perir_sem.simps(1) perir_sem.simps(2) split_pairs)
 
@@ -739,32 +137,114 @@ proof-
     next
       case False
       have b5:"?l!0 \<noteq> 0xe8 \<and> ?l!0 \<noteq> 0xc3" using False b2 by simp
-      then show ?thesis
+      hence bn_1:"?l \<noteq> []" using a8 apply(unfold well_formed_prog_def) using b0 a4 a7 by blast
+      have bn_2:"?num >0 " using a8 apply(unfold well_formed_prog_def) using b0 a4 a7 by blast 
+
+      have c3_0:"list_in_list ?l xpc1 l_bin" using c0 c1 by simp         
+      have c3:"l_bin!xpc1 = ?l!0" using c3_0 bn_1 by (metis list.collapse list_in_list.simps(2) nth_Cons_0)
+      then show ?thesis      
       proof(cases "?l!1 = (0x39::u8)")
+        
         case True
-        hence "xxst' = (let xst_temp = Next 0 xrs xm xss; xst' = x64_sem ?num ?l xst_temp in
+        hence d0:"xxst' = (let xst_temp = Next 0 xrs xm xss; xst' = x64_sem ?num ?l xst_temp in
           case xst' of
           Next xpc' rs' m' ss'\<Rightarrow>
             if rs' (CR ZF) = 1 then (?off+pc, xst')
             else (pc+1, xst') |
           Stuck \<Rightarrow> (pc, Stuck) )" using True b1 b0 b5
           by (smt (z3) case_prod_conv outcome.exhaust outcome.simps(4) outcome.simps(5))  
-        then show ?thesis sorry
+
+        have "l_bin!(xpc1+1) = ?l!1" using c3 c3_0 sorry
+        hence d1:"fxst' = (case x64_sem (snd (l_pc!(unat pc))) l_bin (Next xpc1 xrs xm xss) of
+          Stuck \<Rightarrow> (pc, Stuck) | \<comment>\<open> if one step error, stop, it should be impossible \<close>
+          Next xpc1 rs1 m1 ss1 \<Rightarrow> (
+            if rs1 (CR ZF) = 1 then \<comment>\<open> must JUMP \<close>
+              (case find_target_pc_in_l_pc l_jump pc of
+              None \<Rightarrow> (pc, Stuck) |
+              Some npc \<Rightarrow>
+                (npc, (Next (unat (fst (l_pc!(unat npc)))) rs1 m1 ss1))) \<comment>\<open> go to the target address in the jited x64 binary \<close>
+            else \<comment>\<open> donot JUMP \<close>
+              (pc+1, Next xpc1 rs1 m1 ss1)
+          )) " using True a0 c2 a7 c1 a9 by auto    
+                
+          have "\<exists> fxst1. fxst1 = x64_sem ?num l_bin (Next xpc1 xrs xm xss)" by fastforce
+          then obtain fxst1 where d2_0:"fxst1 = x64_sem ?num l_bin (Next xpc1 xrs xm xss)" by auto
+          have "\<exists> xxst1. xxst1 = x64_sem ?num ?l (Next 0 xrs xm xss)" by fastforce
+          then obtain xxst1 where d2_1:"xxst1 = x64_sem ?num ?l (Next 0 xrs xm xss)" by auto
+          have d2:"match_state1 fxst1 xxst1" using d2_0 d2_1 sorry
+          have d3:"\<exists> xpc' xrs1 xm1 xss1. Next xpc' xrs1 xm1 xss1 = fxst1" 
+            using d2 match_state1_def by (smt (verit, ccfv_threshold) outcome.exhaust outcome.simps(5)) 
+          then obtain xpc' xrs1 xm1 xss1 where d4_0:"Next xpc' xrs1 xm1 xss1 = fxst1" by auto
+          have "\<exists> xpc''. Next xpc'' xrs1 xm1 xss1 = xxst1" 
+            using d3 match_state1_def d4_0 by (smt (verit, ccfv_SIG) d2 outcome.exhaust outcome.simps(4) outcome.simps(5))
+          then obtain xpc'' where d4_1:"Next xpc'' xrs1 xm1 xss1 = xxst1" by auto
+          have d4:"(snd (l_pc!(unat pc))) = ?num"
+            by (metis (mono_tags, lifting) a1 a7 b0 flattern_num) 
+          thus ?thesis
+          proof(cases "xrs1 (CR ZF) = 1")
+            case True
+            have d5_0: "xrs1 (CR ZF) = 1" using True by auto
+            thus ?thesis
+            proof(cases "find_target_pc_in_l_pc l_jump pc \<noteq> None")
+              case True
+                have "\<exists> npc. find_target_pc_in_l_pc l_jump pc = Some npc" using True by simp
+                then obtain npc where d5_1:"find_target_pc_in_l_pc l_jump pc = Some npc" by auto
+                hence d5:"npc = ?off+pc" using a1 a4 b0 a7 flattern_jump_index init_second_layer_def l_jump_upperbound_aux is_increase_list_empty
+                  by (metis (mono_tags, lifting) Abs_fnat_hom_0 add_0 distinct.simps(1) length_0_conv map_is_Nil_conv) 
+                have d6_0:"fxst' =  (npc, (Next (unat (fst (l_pc!(unat npc)))) xrs1 xm1 xss1))" 
+                  using d5_0 d5_1 True d4_0 d1 d2_0 d4 by (smt (verit, best) option.simps(5) outcome.simps(4))
+                have d6_1:"xxst' = (?off+pc, xxst1)"
+                  by (smt (verit, ccfv_threshold) d0 d2_1 d4_1 d5_0 outcome.simps(4)) 
+
+                have "match_state fxst' xxst'" 
+                  using d6_0 d6_1 match_state_def d4_1 d5 match_state1_def by auto
+                then show ?thesis using match_state_def d6_0 d6_1 match_state1_def \<open>\<And>thesis::bool. (\<And>xpc''::nat. Next xpc'' (xrs1::preg \<Rightarrow> 64 word) (xm1::nat \<Rightarrow> int \<Rightarrow> 8 word option) (xss1::stack_state) = (xxst1::outcome) \<Longrightarrow> thesis) \<Longrightarrow> thesis\<close> by fastforce 
+               next
+                 case False
+                 have "find_target_pc_in_l_pc l_jump pc = None" using False by simp
+                 hence "fxst' = (pc,Stuck)" using a9
+                   by (smt (verit, ccfv_SIG) d1 d2_0 d4 d4_0 d5_0 option.case_eq_if outcome.simps(4)) 
+                then show ?thesis using a9 by auto
+              qed
+            next
+              case False
+              have d5_0:"xrs1 (CR ZF) \<noteq> 1" using False by simp
+              have d5_1:"xxst' = (pc+1, xxst1)" by (smt (verit) d0 d2_1 d4_1 d5_0 outcome.simps(4)) 
+              have d5_2:"fxst' = (pc+1, fxst1)" 
+                using d5_0 by (smt (verit, ccfv_threshold) d1 d2_0 d4 d4_0 outcome.simps(4)) 
+            then show ?thesis using d5_1 d5_2 match_state_def d2 d3 d4_1 by force 
+
+        qed
+
+        (*hence bn_0:"x64_decode 0 ?l \<noteq> None" using a6 apply(cases "x64_decode 0 ?l",simp_all) using bn_2
+          by (metis (no_types, lifting) Suc_diff_1 option.simps(4) outcome.simps(5) prod.collapse prod.inject x64_sem.simps(3)) 
+        have bn_3:"x64_decode 0 ?l \<noteq> Some(1,Pret)" using is_ret_insn bn_0 bn_1 
+          by (metis Pair_inject True add_0 is_cmp_insn numeral_eq_one_iff option.sel semiring_norm(86))
+
+        have bn_4:"\<forall> d. x64_decode 0 ?l \<noteq> Some(5, Pcall_i d)"  using is_call_insn bn_0 bn_1 b5 
+          using True is_cmp_insn by fastforce *)
+       
       next
         case False
-        have b6:"?l!0 \<noteq> 0xe8 \<and> ?l!0 \<noteq> 0xc3 \<and> ?l!1 \<noteq> (0x39::u8)" using b5 False by blast
+          have b6:"?l!0 \<noteq> 0xe8 \<and> ?l!0 \<noteq> 0xc3 \<and> ?l!1 \<noteq> (0x39::u8)" using b5 False by blast
           have d0:"xxst' = (let xst_temp = Next 0 xrs xm xss; xst' = x64_sem ?num ?l xst_temp in
           (pc+1, xst'))" using b6 by (smt (verit) b0 b1 case_prod_conv)
           
-          have c3_0:"list_in_list ?l xpc1 l_bin" using c0 c1 by simp
-          have c3_1:"?l \<noteq> []" sorry
-          have c3:"l_bin!xpc1 = ?l!0" using c3_0 c3_1
-            by (metis list_in_list.simps(2) list_in_list_prop neq_Nil_conv) 
-           (* by (metis list.collapse list_in_list.simps(2)) *)
-          have c3_2:"l_bin!(xpc1+1) \<noteq> (0x39::u8)" sorry
+          hence bn_0:"x64_decode 0 ?l \<noteq> None" using d0 a6 bn_2 apply(cases "x64_decode 0 ?l",simp_all)
+            by (smt (verit) Suc_diff_1 option.simps(4) x64_sem.simps(3))
+          hence "x64_decode 0 ?l \<noteq> Some(1,Pret) \<and> (\<forall> d. x64_decode 0 ?l \<noteq> Some(5, Pcall_i d)) \<and> (\<forall> src dst. x64_decode 0 ?l \<noteq> Some(3, Pcmpq_rr src dst))"
+            using not_ret_insn not_call_insn not_cmp_insn bn_1 b6 by simp
+
+          (*have bn_3:"x64_decode 0 ?l \<noteq> Some(1,Pret)" using is_ret_insn bn_0 bn_1 b6          
+
+          have bn_4:"\<forall> d. x64_decode 0 ?l \<noteq> Some(5, Pcall_i d)"  using is_call_insn bn_0 bn_1 b5
+          using True is_cmp_insn by fastforce *)
+                   
+        
+          have c3_2:"l_bin!(xpc1+1) \<noteq> (0x39::u8)" using c3 c3_0 sorry
           
           have c4:"fxst' = (let num = snd (l_pc!(unat pc)) in (pc+1, x64_sem num l_bin (Next xpc1 xrs xm xss)))"
-            using c2 c3 b6 c3_2 by presburger 
+            using c2 b6 c3_2 a1 a7 add.right_neutral c1 init_second_layer_def l_pc_length_prop a9 by force 
           have c5_1:"l_pc \<noteq> []"  using a1 a4 apply(unfold init_second_layer_def) using num_corr by fastforce 
 
           have c5:"fxst' = (pc+1, x64_sem ?num l_bin (Next xpc1 xrs xm xss))"using b0 c5_1 a1 init_second_layer_def c4 a6 a7
@@ -822,7 +302,7 @@ lemma intermediate_step_is_ok:"perir_sem n lt (pc,s) = s' \<Longrightarrow> n \<
   by (metis JITFlattern.err_is_still_err outcome.exhaust prod.collapse) 
 
 
-lemma n_steps_equiv:
+lemma n_steps_equiv_layer1:
   "flat_bpf_sem n prog (pc,fxst) = fxst' \<Longrightarrow>
   jitflat_bpf lt init_second_layer = prog \<Longrightarrow>
   perir_sem n lt (pc,xxst) = xxst' \<Longrightarrow>
@@ -830,9 +310,10 @@ lemma n_steps_equiv:
   snd xxst' = Next xpc' xrs' xm' xss' \<Longrightarrow>
   match_state (pc,xxst) (pc,fxst) \<Longrightarrow>
   lt \<noteq> [] \<Longrightarrow> 
-  unat pc < length lt \<and> unat pc \<ge> 0 \<Longrightarrow>
+  well_formed_prog lt \<Longrightarrow>
+  snd fxst' = Next xpc'' xrs'' xm'' xss'' \<Longrightarrow>
   match_state xxst' fxst'"
-proof(induct n arbitrary: prog pc fxst fxst' lt xxst xxst' xpc xrs xm xss xxst' xpc' xrs' xm' xss')
+proof(induct n arbitrary: prog pc fxst fxst' lt xxst xxst' xpc xrs xm xss xxst' xpc' xrs' xm' xss' xpc'' xrs'' xm'' xss'')
   case 0
   then show ?case apply(unfold match_state_def,simp_all) 
     done
@@ -846,7 +327,10 @@ next
   assm4:"snd xxst' = Next xpc' xrs' xm' xss'" and
   assm5:"lt \<noteq> []" and
   assm6:"match_state (pc,xxst) (pc,fxst)" and
-  assm7:"unat pc < length lt \<and> unat pc \<ge> 0"
+(*  assm7:"unat pc < length lt \<and> unat pc \<ge> 0" and*)
+  assm7:"well_formed_prog lt" and
+  assm8:"snd fxst' = Next xpc'' xrs'' xm'' xss''"
+ 
   have "\<exists> next_s. next_s = perir_sem 1 lt (pc,xxst)" by simp
   then obtain next_s pc' where b0:"next_s = perir_sem 1 lt (pc,xxst)" by auto
   have "\<exists> next_f. flat_bpf_sem 1 prog (pc,fxst) = next_f" by blast
@@ -856,12 +340,24 @@ next
     done*)
   have a0:"perir_sem n lt next_s = xxst'" using x64_sem1_induct_aux3 assm2 b0
     using Suc.prems(3) by presburger 
-  have "\<exists> pc' xrs1 xpc1 m1 xss1. (pc', Next xrs1 xpc1 m1 xss1) = next_s" using assm4 a0 intermediate_step_is_ok a0
+  have "\<exists> pc' xrs1 xpc1 m1 xss1. (pc', Next xrs1 xpc1 m1 xss1) = next_s" using assm4 a0 intermediate_step_is_ok
     by (metis outcome.exhaust prod.collapse zero_le) 
   then obtain pc' xrs1 xpc1 m1 xss1 where a1:"(pc', Next xrs1 xpc1 m1 xss1) = next_s" by auto
-  
+                                                                                                            
+  (*have "\<exists> pc'' xrs1' xpc1' m1' xss1'. (pc'', Next xrs1' xpc1' m1' xss1') = next_f" using assm8 intermediate_step_is_ok3 b1
+    by (metis Suc.prems(9) assm0 bot_nat_0.extremum flat_bpf_sem_induct_aux2 outcome.distinct(1) prod.exhaust_sel) *)
+  have c0_1:"snd next_f \<noteq> Stuck" using assm8 intermediate_step_is_ok3 b1
+    by (metis assm0 bot_nat_0.extremum flat_bpf_sem_induct_aux2 outcome.distinct(1) prod.exhaust_sel) 
+
+  hence"(unat pc < length (fst(snd prog)) \<and> unat pc \<ge> 0)" using b1 assm8
+    by (smt (z3) One_nat_def case_prod_conv flat_bpf_one_step_def flat_bpf_sem.simps(1) flat_bpf_sem.simps(2) 
+        intermediate_step_is_ok3 linorder_not_less outcome.simps(4) prod.collapse split_pairs zero_order(1)) 
+
+  hence c0:"(unat pc < length lt \<and> unat pc \<ge> 0)" using l_pc_length_prop  init_second_layer_def assm1
+    by (metis add.right_neutral list.size(3) prod.collapse) 
   have bn:"match_state next_s next_f"
-    using one_step_equiv b1 assm1 b0 assm3 assm5 assm6 a1 assm7 by (metis eq_snd_iff outcome.distinct(1)) 
+    using one_step_equiv_layer1 b1 assm1 b0 assm3 assm5 assm6 a1 c0 assm8 c0_1 assm7
+    by (metis outcome.distinct(1) prod.collapse snd_conv) 
 
   have a2:"(pc', snd next_f) = next_f" using bn match_state_def a1 b0 b1
     apply(cases "Next xrs1 xpc1 m1 xss1",simp_all)
@@ -870,14 +366,13 @@ next
     subgoal for x11 by force
     done
 
-  have c0:"flat_bpf_sem n prog next_f = fxst'" using flat_bpf_sem_induct_aux2 assm0 b1 by blast
+  have c1:"flat_bpf_sem n prog next_f = fxst'" using flat_bpf_sem_induct_aux2 assm0 b1 by blast
 
-  have "unat pc' < length lt \<and> unat pc \<ge> 0" sorry
   hence "match_state xxst' fxst'" 
-    using a0 a1 a2 Suc bn c0 assm5 assm4 assm7 by (metis bot_nat_0.extremum) 
+    using a0 a1 a2 Suc bn c1 assm5 assm4 by metis
   then show ?case by simp
 qed
 
-
+  
 
 end
