theory/JITFlattern_def.thy
@@ -1,0 +1,106 @@
+theory JITFlattern_def
+  imports JITPer
+begin
+type_synonym flat_bpf_prog = "x64_bin \<times> (u64 \<times> nat) list \<times> ((u64\<times>u64) list)"
+
+definition update_l_jump::"(nat \<times> u64 \<times> x64_bin) \<Rightarrow> (u64 \<times> nat) list \<Rightarrow> (u64\<times>u64) list \<Rightarrow> (u64\<times>u64) list" where
+"update_l_jump x l_pc l_jump \<equiv> let (num,off,l_bin0) = x in 
+  if l_bin0!1 = (0x39::u8) then l_jump@ [(of_nat (length l_pc), of_nat (length l_pc) + off)]
+  else l_jump"
+
+fun jitflat_bpf :: "(nat \<times> u64 \<times> x64_bin) list \<Rightarrow> flat_bpf_prog \<Rightarrow> flat_bpf_prog" where
+"jitflat_bpf [] st = st"| 
+"jitflat_bpf ((num,off,l_bin0)#xs) (l_bin,l_pc,l_jump) = (
+  let curr_pc = of_nat (length l_bin) in 
+  let l_jump' = update_l_jump (num,off,l_bin0) l_pc l_jump in
+      jitflat_bpf xs (
+        l_bin@l_bin0,
+        l_pc@[(curr_pc,num)],
+        l_jump')
+)"
+
+definition init_second_layer::"x64_bin \<times> (u64 \<times> nat) list \<times> ((u64\<times>u64) list)" where
+"init_second_layer \<equiv> ([],[],[])"
+
+(*fun well_formed_prog_aux::"(nat \<times> u64 \<times> x64_bin) list \<Rightarrow> bool" where
+  "well_formed_prog_aux [] = True" |
+  "well_formed_prog_aux (x#xs) = (let (num,off,l) = x in 
+    num > 0 \<and> l \<noteq> [] \<and> well_formed_prog_aux xs)"
+
+
+value "well_formed_prog_aux [(1,0,[3])]"
+  
+definition well_formed_prog::"(nat \<times> u64 \<times> x64_bin) list \<Rightarrow> bool" where
+"well_formed_prog lt \<equiv> well_formed_prog_aux lt \<and> length lt \<le> 100000 \<and> lt \<noteq> []"
+
+value "well_formed_prog [(1,0,[3])]"*)
+
+definition well_formed_prog::"(nat \<times> u64 \<times> x64_bin) list \<Rightarrow> bool" where
+"well_formed_prog lt \<equiv> (length lt \<le> 100000 \<and> lt \<noteq> [] \<and> 
+  (\<forall> id. id < length lt \<and> id \<ge>0 \<longrightarrow> snd(snd (lt!id)) \<noteq> [] \<and> fst(lt!id) >0) \<and>
+  (\<forall> idx. idx \<ge> 0 \<and> idx < length (map snd (map snd lt)) \<longrightarrow> length ((map snd (map snd lt))!idx) \<le> 10))"
+
+fun find_target_pc_in_l_pc :: "((u64\<times>u64) list) \<Rightarrow> u64 \<Rightarrow> u64 option" where
+"find_target_pc_in_l_pc [] _ = None" |
+"find_target_pc_in_l_pc ((x, y)#xs) pc = (
+  if x = pc then Some y
+  else find_target_pc_in_l_pc xs pc
+)"
+
+(*if unat pc \<ge> length lp \<or> unat pc < 0 then (pc,Stuck) else *)
+definition flat_bpf_one_step :: "flat_bpf_prog \<Rightarrow> hybrid_state \<Rightarrow> hybrid_state" where
+"flat_bpf_one_step lp st = (
+  let (l_bin,l_pc,l_jump) = lp in
+  let (pc, xst) = st in
+    (case xst of
+    Stuck \<Rightarrow> (pc, Stuck) |
+    Next xpc rs m ss \<Rightarrow> (
+    if unat pc \<ge> length l_pc \<or> unat pc < 0 then (pc,Stuck) else 
+    let num = snd (l_pc!(unat pc)) in 
+    let old_xpc = unat (fst (l_pc!(unat pc))) in 
+      if xpc \<noteq> old_xpc then (pc, Stuck) else 
+        if l_bin!(xpc+1) = (0x39::u8) then \<comment>\<open> TODO: if the first byte is the opcode of cmp? \<close>
+          \<comment>\<open> case: BPF JMP \<close>
+          (case x64_sem num l_bin (Next xpc rs m ss) of
+          Stuck \<Rightarrow> (pc, Stuck) | \<comment>\<open> if one step error, stop, it should be impossible \<close>
+          Next xpc1 rs1 m1 ss1 \<Rightarrow> (
+            if rs1 (CR ZF) = 1 then \<comment>\<open> must JUMP \<close>
+              (case find_target_pc_in_l_pc l_jump pc of
+              None \<Rightarrow> (pc, Stuck) |
+              Some npc \<Rightarrow>
+                (npc, (Next (unat (fst (l_pc!(unat npc)))) rs1 m1 ss1))) \<comment>\<open> go to the target address in the jited x64 binary \<close>
+            else \<comment>\<open> donot JUMP \<close>
+              (pc+1, (Next xpc1 rs1 m1 ss1))
+          ))
+         else
+          \<comment>\<open> case: NOT BPF JMP \<close>
+          (pc+1, x64_sem num l_bin (Next xpc rs m ss))
+)))"
+
+fun flat_bpf_sem :: "nat \<Rightarrow> flat_bpf_prog \<Rightarrow> hybrid_state \<Rightarrow> hybrid_state" where
+"flat_bpf_sem 0 _ (pc,st) = (pc,st)" |
+"flat_bpf_sem (Suc n) lt (pc, xst) = (
+   let pair = flat_bpf_one_step lt (pc, xst) in
+    flat_bpf_sem n lt pair
+)"
+
+definition match_state1::"outcome \<Rightarrow> outcome \<Rightarrow> bool" where
+  "match_state1 fxst xxst \<equiv> 
+  (case fxst of (Next xst xrs xm xss) \<Rightarrow>
+    (case xxst of (Next xst1 xrs1 xm1 xss1) \<Rightarrow> 
+     xrs = xrs1 \<and> xm = xm1 \<and> xss = xss1 |
+                   _ \<Rightarrow> False)|
+                 _ \<Rightarrow> False)"
+
+definition match_state::"hybrid_state \<Rightarrow> hybrid_state \<Rightarrow> bool" where
+  "match_state fxst xxst \<equiv> 
+  (case fxst of (pc,Next xst xrs xm xss) \<Rightarrow>
+    (case xxst of (pc1,Next xst1 xrs1 xm1 xss1) \<Rightarrow> 
+      pc = pc1 \<and> match_state1 (Next xst1 xrs1 xm1 xss1) (Next xst xrs xm xss)  |
+                   _ \<Rightarrow> False)|
+                 _ \<Rightarrow> False)"
+(*x64_decode 0 l = x64_decode xpc l
+xxst = Next xpc1 xrs1 xm1 xss1 \<Longrightarrow>
+   fxst = Next xpc2 xrs2 xm2 xss2 \<Longrightarrow>
+xrs1 = xrs2 \<and> xm1 = xm2 \<and> xss1 = xss2*)
+end
